

Factor each of the following expressions.

(a)  $x^{2/3} - 2x^{1/3}$

(b)  $\ln x - e^x \ln x$

(c)  $\sin x \cos x + \cos x$

(d)  $e^{2x} - 2e^x + 1$

(e)  $3(x+2)^2(3x-4)^{-2} + (x+2)^3(-2)(3x-4)^{-3}(3)$

**Solutions on the next page**

(a)  $x^{2/3} - 2x^{1/3} = x^{1/3}(x^{1/3} - 2)$

This expression has two terms. We first look for common factors, and here we see an  $x$  in each term.

**We want to factor out the smallest power of  $x$ .** In this case,  $1/3 < 2/3$ , so we factor out  $x^{1/3}$ .

$$x^{2/3} - 2x^{1/3} = x^{1/3}(x^? - 2)$$

To determine what goes in place of  $?$ , we must calculate  $\frac{x^{2/3}}{x^{1/3}}$ , which simplifies to  $x^{1/3}$  using laws of exponents. is the smallest power of  $x$  contained in both terms, and  $x^{1/3} \cdot x^{1/3} = x^{2/3}$ .

$$x^{2/3} - 2x^{1/3} = x^{1/3}(x^{1/3} - 2)$$

Note that if we distribute  $x^{1/3}$  to both terms, we get back to where we started.

(b)  $\ln x - e^x \ln x = (\ln x)(1 - e^x)$

Here, we just notice that both terms contain a factor of  $\ln x$ , and we factor it out of both terms:

$$\ln x - e^x \ln x = (\ln x)(1 - e^x)$$

Again, distributing would result in the expression we started with.

(c)  $\sin x \cos x + \cos x = (\cos x)(\sin x + 1)$

Again, here we just see the common factor of  $\cos x$  in each term.

$$\sin x \cos x + \cos x = (\cos x)(\sin x + 1)$$

(d)  $e^{2x} - 2e^x + 1 = (e^x - 1)(e^x - 1) = (e^x - 1)^2$

The expression is in quadratic form, because  $e^{2x} = (e^x)^2$ . If we substitute  $u = e^x$ , we get

$$e^{2x} - 2e^x + 1 = (e^x)^2 - 2e^x + 1 = u^2 - 2u + 1$$

Now we can factor the  $u$  version of the expression:

$$u^2 - 2u + 1 = (u - 1)(u - 1)$$

Substituting  $u = e^x$  back in, we see

$$e^{2x} - 2e^x + 1 = (u - 1)(u - 1) = (e^x - 1)(e^x - 1)$$

(e)  $3(x + 2)^2(3x - 4)^{-2} + (x + 2)^3(-2)(3x - 4)^{-3}(3) = 3(x + 2)^2(3x - 4)^{-3}(x - 8)$

This expression has two monster terms in it. Each of the two monster terms contains a factor of 3, some power of  $x + 2$ , and some power of  $3x - 4$ .

The smallest exponent on  $x + 2$  is 2, so we factor out  $(x + 2)^2$ .

The smallest exponent on  $3x - 4$  is  $-3$  (remember  $-3 < -2$ ), so we factor out  $(3x - 4)^{-3}$ .

We will be left with two terms.

$$3(x + 2)^2(3x - 4)^{-2} + (x + 2)^3(-2)(3x - 4)^{-3}(3) = 3(x + 2)^2(3x - 4)^{-3} [ \quad + \quad ]$$

To determine what goes in brackets, we take each initial term and divide by what we have factored out, using laws of exponents to simplify.

$$\frac{3(x+2)^2(3x-4)^{-2}}{3(x+2)^2(3x-4)^{-3}} = \frac{(3x-4)^{-2}}{(3x-4)^{-3}} = (3x-4)^{-2-(-3)} = (3x-4)^1 = 3x-4$$

$$\frac{(x+2)^3(-2)(3x-4)^{-3}(3)}{3(x+2)^2(3x-4)^{-3}} = \frac{(x+2)^3(-2)}{(x+2)^2} = (-2)(x+2)^1 = -2x-4$$

Filling in the brackets:

$$3(x+2)^2(3x-4)^{-2} + (x+2)^3(-2)(3x-4)^{-3}(3) = 3(x+2)^2(3x-4)^{-3} [(3x-4) + (-2x-4)]$$

We can check that if we expand the expression on the right, we get back to where we started. And now combining what is in the brackets:

$$3(x+2)^2(3x-4)^{-2} + (x+2)^3(-2)(3x-4)^{-3}(3) = 3(x+2)^2(3x-4)^{-3}(x-8)$$